Xv6/SpecKfork.lean
@@ -87,12 +87,12 @@ def wp_kfork_body {hlc : HasLC} {GF : BundledGFunctors} [MachGS hlc GF] [Xv6G GF
   isLock γw waitLockAddr "wait_lock" waitLockPay ∗
   isLock γp pidLockAddr "nextpid" pidLockPay ∗
   isLock γl kmemLockAddr "kmem" (kmemRes γk) ∗ kallocAvail γk none ∗
-  procPriv (procAddr j) pid V M ∗
+  procPrivNoctxAt curCtx (procAddr j) pid V M ∗
   wpNext true k.proc cpu (fun cpu' => iprop(∀ (spie spp : Bool) (R' : RegMap) (rv : BitVec 32),
     ⌜calleeSaved k.regs R' ∧ R' 10#5 = BitVec.signExtend 64 rv ∧ kforkAns rv⌝ -∗
     kctx cpu' ((k.withSpie spie spp).withRegs R') -∗ pcIs cpu' (jumpPc (k.regs 1#5)) -∗
     trapCsrs cpu' -∗ cpuClaim cpu' k.proc -∗ intrRes cpu' -∗
-    procPriv (procAddr j) pid V M -∗ wpLoop cpu'))
+    procPrivNoctxAt curCtx (procAddr j) pid V M -∗ wpLoop cpu'))
   ⊢ wpLoop (GF := GF) cpu
 
 /-- The interface of `kfork`. -/
