Xv6/SpecKwait.lean
@@ -102,14 +102,14 @@ def wp_kwait_body {hlc : HasLC} {GF : BundledGFunctors} [MachGS hlc GF] [Xv6G GF
   isLock γw waitLockAddr "wait_lock" waitLockPay ∗
   isLock γp pidLockAddr "nextpid" pidLockPay ∗
   isLock γl kmemLockAddr "kmem" (kmemRes γk) ∗ kallocAvail γk none ∗
-  procPriv (procAddr j) pid V M ∗
+  procPrivNoctxAt curCtx (procAddr j) pid V M ∗
   wpNext true k.proc cpu (fun cpu' => iprop(∀ (spie spp : Bool) (R' : RegMap) (P' : UPtd)
     (rv xw : BitVec 32) (d : Nat),
     ⌜calleeSaved k.regs R' ∧ R' 10#5 = BitVec.signExtend 64 rv ∧ V.upt.ext P' ∧ d ≤ 4 ∧
       kwaitAns rv (k.regs 10#5) d⌝ -∗
     kctx cpu' ((k.withSpie spie spp).withRegs R') -∗ pcIs cpu' (jumpPc (k.regs 1#5)) -∗
     trapCsrs cpu' -∗ cpuClaim cpu' k.proc -∗ intrRes cpu' -∗
-    procPrivExt (procAddr j) pid V P'
+    procPrivExtNoctxAt curCtx (procAddr j) pid V P'
       (umemWrite (viewFaulted V.upt P' M) (k.regs 10#5).toNat ((xstateBytes xw).take d)) -∗
     wpLoop cpu'))
   ⊢ wpLoop (GF := GF) cpu
